Remove Array4, just a special case of tensor

src/lib/data/Kuiper.Matrix.Casts.fst
@@ -5,13 +5,12 @@ open Kuiper
 
 open Kuiper.Tensor
 module A2 = Kuiper.Array2
-module A4 = Kuiper.Array4
 open Kuiper.EMatrix
 open Kuiper.EMatrix4
 
 // TODO: define this by composing a bijection with the l.imap injection
 #push-options "--z3rlimit 20 --retry 3"
-let l2_to_l4 (#m #n : nat) (#mm #nn : pos) (l : A2.layout (m * mm) (n * nn)) : A4.layout m n mm nn = {
+let l2_to_l4 (#m #n : nat) (#mm #nn : pos) (l : layout2 (m * mm) (n * nn)) : layout4 m n mm nn = {
   ulen = l.ulen;
   imap =
     Kuiper.Injection.mk_injection
@@ -34,7 +33,7 @@ let em2_to_em4 (#et : Type0) (#m #n #mm #nn : nat) (e : ematrix et (m * mm) (n *
   Kuiper.EMatrix4.mkM (fun i j k o -> Kuiper.EMatrix.macc e (i * mm + k) (j * nn + o))
 
 #push-options "--z3rlimit 20 --retry 3"
-let l4_to_l2 (#m #n : nat) (#mm #nn : pos) (l : A4.layout m n mm nn) : A2.layout (m * mm) (n * nn) = {
+let l4_to_l2 (#m #n : nat) (#mm #nn : pos) (l : layout4 m n mm nn) : layout2 (m * mm) (n * nn) = {
   ulen = l.ulen;
   imap =
     Kuiper.Injection.mk_injection #(natlt (m * mm) & (natlt (n * nn) & unit))
@@ -78,16 +77,16 @@ fn m2_to_m4
   requires
     gA |-> Frac f eA
   returns
-    gA4 : A4.t et (l2_to_l4 lA)
+    gA4 : array4 et (l2_to_l4 lA)
   ensures
     gA4 |-> Frac f (em2_to_em4 eA) **
-    pure (A4.core gA4 == A2.core gA)
+    pure (core gA4 == A2.core gA)
 {
   (* Very roundabout way to do this. *)
   A2.lower gA;
-  A4.raise' (l2_to_l4 lA) (A2.core gA);
-  let r = A4.from_array (l2_to_l4 lA) (A2.core gA);
-  assert rewrites_to r (A4.from_array (l2_to_l4 lA) (A2.core gA));
+  tensor_abs' (l2_to_l4 lA) (A2.core gA);
+  let r = from_array (l2_to_l4 lA) (A2.core gA);
+  assert rewrites_to r (from_array (l2_to_l4 lA) (A2.core gA));
   assert pure (Kuiper.EMatrix4.equal
     (from_seq (l2_to_l4 lA) (to_seq lA eA))
     (em2_to_em4 eA));
@@ -101,8 +100,8 @@ inline_for_extraction noextract
 fn m4_to_m2
   (m n mm nn : erased nat{mm > 0 /\ nn > 0})
   (#et : Type0) {| scalar et |}
-  (#lA4 : A4.full_layout m n mm nn)
-  (gA4 : A4.t et lA4)
+  (#lA4 : full_layout4 m n mm nn)
+  (gA4 : array4 et lA4)
   (#eA4 : ematrix4 et _ _ _ _)
   (#f : perm)
   requires
@@ -111,13 +110,13 @@ fn m4_to_m2
     gA : A2.t et (l4_to_l2 lA4)
   ensures
     gA |-> Frac f (em4_to_em2 eA4) **
-    pure (A4.core gA4 == A2.core gA)
+    pure (core gA4 == A2.core gA)
 {
   (* Very roundabout way to do this. *)
-  A4.lower gA4;
-  A2.raise' (l4_to_l2 lA4) (A4.core gA4);
-  let r = A2.from_array (l4_to_l2 lA4) (A4.core gA4);
-  assert rewrites_to r (A2.from_array (l4_to_l2 lA4) (A4.core gA4));
+  tensor_concr gA4;
+  A2.raise' (l4_to_l2 lA4) (core gA4);
+  let r = A2.from_array (l4_to_l2 lA4) (core gA4);
+  assert rewrites_to r (A2.from_array (l4_to_l2 lA4) (core gA4));
   assert pure (Kuiper.EMatrix.equal
     (from_seq (l4_to_l2 lA4) (to_seq lA4 eA4))
     (em4_to_em2 eA4));
